q

Generic_ZK.ec
@@ -7,49 +7,57 @@ require import Aux.
 type prob, wit, chal, com, resp, sbits, event, auxiliary_input.
 
 require While_Props.
-clone import While_Props as MW with type irt   <- prob,
+clone import While_Props as MW with type irt   <- prob * auxiliary_input,
                                     type rrt   <- event * sbits,
                                     type sbits <- sbits.
 import MW.IFB.
 import MW.IFB.IM.
 
 
-
-module type Simulator = {
-  proc run(Ny : prob) : event * sbits
-}.
-
 module type Dist = {
-  proc run(_:prob * wit * auxiliary_input * event * sbits) : bool
+  proc run(_:prob * wit * auxiliary_input * sbits) : bool
+}.
+
+module type MaliciousVerifier = {
+  proc challenge(statement: prob, aux: auxiliary_input) : chal
+  proc summitup(statement: prob, response: resp) : sbits
 }.
 
 
-module W0(Sim1:Simulator, D : Dist) = {
+
+
+module type Simulator1(V : MaliciousVerifier) = {
+  proc run(Ny : prob, aux : auxiliary_input) : event * sbits
+}.
+
+
+module W0(Sim1:Simulator1, V : MaliciousVerifier, D : Dist) = {
+  module Sim1 = Sim1(V)
   proc run(a : prob, w : wit, aux : auxiliary_input) = {
       var r, b;
-      r <- Sim1.run(a);
-      b <- D.run(a,w,aux,r.`1,r.`2);
+      r <- Sim1.run(a,aux);
+      b <- D.run(a,w,aux,r.`2);
       return (b, r);
   }
 }.
 
 
-module W1(Sim1:Simulator, D : Dist) = {
-  module M = W(Sim1)
-  proc run(a : (event * sbits -> bool) * prob * int * int * (event * sbits), w : wit, aux : auxiliary_input) = {
+module W1(Sim1:Simulator1, V : MaliciousVerifier, D : Dist) = {
+  module M = W(Sim1(V))
+  proc run(a : (event * sbits -> bool) * (prob * auxiliary_input) * int * int * (event * sbits), w : wit) = {
       var r, b;
       r <- M.whp(a);
-      b <- D.run(a.`2,w,aux,r.`1,r.`2);
+      b <- D.run(a.`2.`1,w,a.`2.`2, r.`2);
       return (b, r);
   }
 }.
 
 
-module Iter(Sim1 : Simulator, D : Dist)  = {
-  module WI = W1(Sim1,D)
+module Iter(Sim1 : Simulator1, V : MaliciousVerifier, D : Dist)  = {
+  module WI = W1(Sim1,V,D)
   proc run(fevent : event, Ny : prob, w : wit, aux : auxiliary_input, ea : int, E : event * sbits -> bool) = {
     var r;
-    r <@ WI.run((E,Ny,1,ea,(fevent,witness)),w,aux);
+    r <@ WI.run((E,(Ny,aux),1,ea,(fevent,witness)),w);
     return r;
   }
 }.
@@ -58,11 +66,11 @@ module Iter(Sim1 : Simulator, D : Dist)  = {
 
 
 section.
+declare module V : MaliciousVerifier{DW,W}.
+declare module Sim1 : Simulator1{DW, W,V}.
+declare module D : Dist {Sim1,V,W}.
 
-declare module Sim1 : Simulator{DW, W}.
-declare module D : Dist {Sim1}.
-
-axiom Sim1_ll : islossless Sim1.run.
+axiom Sim1_ll : islossless Sim1(V).run.
 axiom D_ll    : islossless D.run.
 
 op fevent : event.
@@ -71,21 +79,21 @@ axiom  Estart :  E (fevent, witness) = false.
 
 
 local lemma zk_step1 &m E p eps zkp:
-   `|Pr[ W0(Sim1, D).run(p) @ &m : E res.`2 /\ res.`1]
-      / Pr[W0(Sim1, D).run(p) @ &m : E res.`2] 
+   `|Pr[ W0(Sim1, V, D).run(p) @ &m : E res.`2 /\ res.`1]
+      / Pr[W0(Sim1, V, D).run(p) @ &m : E res.`2] 
         - zkp| <= eps
   => 0%r <= eps 
-  => 0%r < Pr[W0(Sim1,D).run(p) @ &m : E res.`2]
+  => 0%r < Pr[W0(Sim1,V,D).run(p) @ &m : E res.`2]
   => exists (eps' : real),  0%r <= eps' <= eps  
-  /\ `|Pr[ W0(Sim1,D).run(p) @ &m : E res.`2 /\ res.`1] 
-         / Pr[W0(Sim1,D).run(p) @ &m : E res.`2] 
+  /\ `|Pr[ W0(Sim1,V,D).run(p) @ &m : E res.`2 /\ res.`1] 
+         / Pr[W0(Sim1,V,D).run(p) @ &m : E res.`2] 
                 - zkp| = eps'
-  /\ (Pr[ W0(Sim1,D).run(p) @ &m : E res.`2 /\ res.`1] 
-      = Pr[W0(Sim1,D).run(p) @ &m : E res.`2]  
+  /\ (Pr[ W0(Sim1,V,D).run(p) @ &m : E res.`2 /\ res.`1] 
+      = Pr[W0(Sim1,V,D).run(p) @ &m : E res.`2]  
         * (zkp - eps')
       \/
-      Pr[ W0(Sim1,D).run(p) @ &m : E res.`2 /\ res.`1] 
-      = Pr[W0(Sim1,D).run(p) @ &m : E res.`2]  
+      Pr[ W0(Sim1,V,D).run(p) @ &m : E res.`2 /\ res.`1] 
+      = Pr[W0(Sim1,V,D).run(p) @ &m : E res.`2]  
         * (zkp + eps')).
 proof.
 progress.
@@ -95,41 +103,41 @@ qed.
 
 
 local lemma zk_step2 &m E p ea w aux :
-  Pr[ W1(Sim1,D).run((E,p,1,ea,(fevent,witness)),w,aux) 
+  Pr[ W1(Sim1,V,D).run((E,(p,aux),1,ea,(fevent,witness)),w) 
            @ &m : E res.`2 /\ res.`1 ]  
      = big predT
-        (fun i => Pr[W0(Sim1,D).run(p,w,aux) @ &m : !E res.`2] ^ i 
-         * Pr[ W0(Sim1,D).run(p,w,aux) @ &m : E res.`2 /\  res.`1] )
+        (fun i => Pr[W0(Sim1,V,D).run(p,w,aux) @ &m : !E res.`2] ^ i 
+         * Pr[ W0(Sim1,V,D).run(p,w,aux) @ &m : E res.`2 /\  res.`1] )
         (range 0 ea). 
 admitted.
 
 
 local lemma zk_step3 &m p eps ea coeff zkp (w : wit) aux:
-   `|Pr[ W0(Sim1,D).run(p,w,aux) @ &m : E res.`2 /\ res.`1]
-      / Pr[W0(Sim1,D).run(p,w,aux) @ &m : E res.`2] 
+   `|Pr[ W0(Sim1,V,D).run(p,w,aux) @ &m : E res.`2 /\ res.`1]
+      / Pr[W0(Sim1,V,D).run(p,w,aux) @ &m : E res.`2] 
         - zkp| <= eps
-  => 0%r < Pr[W0(Sim1,D).run(p,w,aux) @ &m : E res.`2]  
+  => 0%r < Pr[W0(Sim1,V,D).run(p,w,aux) @ &m : E res.`2]  
   => 0%r <= eps 
   => coeff = big predT
-               (fun i => Pr[W0(Sim1,D).run(p,w,aux) @ &m : !E res.`2] ^ i 
-                          * Pr[ W0(Sim1,D).run(p,w,aux) @ &m : E res.`2])
+               (fun i => Pr[W0(Sim1,V,D).run(p,w,aux) @ &m : !E res.`2] ^ i 
+                          * Pr[ W0(Sim1,V,D).run(p,w,aux) @ &m : E res.`2])
                (range 0 ea) 
   => exists (eps' : real), 
     0%r <= eps' <= eps   /\ 
-     `|Pr[ W1(Sim1,D).run((E,p,1,ea,(fevent,witness)), w, aux   ) 
+     `|Pr[ W1(Sim1,V,D).run((E,(p,aux),1,ea,(fevent,witness)), w   ) 
            @ &m : E res.`2 /\ res.`1 ]  
          - coeff * zkp| = coeff * eps'.
 proof. move => H0 H1 H2 coeffeq.
 have :  exists (eps' : real),  0%r <= eps' <= eps  
-  /\ `|Pr[ W0(Sim1,D).run(p,w,aux) @ &m : E res.`2 /\ res.`1] 
-         / Pr[W0(Sim1,D).run(p,w,aux) @ &m : E res.`2] 
+  /\ `|Pr[ W0(Sim1,V,D).run(p,w,aux) @ &m : E res.`2 /\ res.`1] 
+         / Pr[W0(Sim1,V,D).run(p,w,aux) @ &m : E res.`2] 
                 - zkp| = eps'
-  /\ (Pr[ W0(Sim1,D).run(p,w,aux) @ &m : E res.`2 /\ res.`1] 
-      = Pr[W0(Sim1,D).run(p,w,aux) @ &m : E res.`2]  
+  /\ (Pr[ W0(Sim1,V,D).run(p,w,aux) @ &m : E res.`2 /\ res.`1] 
+      = Pr[W0(Sim1,V,D).run(p,w,aux) @ &m : E res.`2]  
         * (zkp - eps')
       \/
-      Pr[ W0(Sim1,D).run(p,w,aux) @ &m : E res.`2 /\ res.`1] 
-      = Pr[W0(Sim1,D).run(p,w,aux) @ &m : E res.`2]  
+      Pr[ W0(Sim1,V,D).run(p,w,aux) @ &m : E res.`2 /\ res.`1] 
+      = Pr[W0(Sim1,V,D).run(p,w,aux) @ &m : E res.`2]  
         * (zkp + eps')).
 apply (zk_step1 &m). assumption. assumption. assumption.
 elim. move => eps' [H3 [H41 H42 ]].
@@ -137,31 +145,31 @@ exists eps'.
 split. auto.
 apply oip4.
 rewrite coeffeq.
-have ->: Pr[W0(Sim1,D).run(p,w,aux) @ &m : ! E res.`2]
-  = 1%r - Pr[W0(Sim1,D).run(p,w,aux) @ &m :  E res.`2].
-  have ->: 1%r = Pr[W0(Sim1,D).run(p,w,aux) @ &m :  true].
+have ->: Pr[W0(Sim1,V,D).run(p,w,aux) @ &m : ! E res.`2]
+  = 1%r - Pr[W0(Sim1,V,D).run(p,w,aux) @ &m :  E res.`2].
+  have ->: 1%r = Pr[W0(Sim1,V,D).run(p,w,aux) @ &m :  true].
   byphoare. 
 proc. call D_ll. call Sim1_ll. auto. auto. auto.
-  have ->: Pr[W0(Sim1,D).run(p,w,aux) @ &m : true] = Pr[W0(Sim1,D).run(p,w,aux) @ &m : E res.`2]
-   + Pr[W0(Sim1,D).run(p,w,aux) @ &m : !E res.`2]. rewrite Pr[mu_split E res.`2]. 
+  have ->: Pr[W0(Sim1,V,D).run(p,w,aux) @ &m : true] = Pr[W0(Sim1,V,D).run(p,w,aux) @ &m : E res.`2]
+   + Pr[W0(Sim1,V,D).run(p,w,aux) @ &m : !E res.`2]. rewrite Pr[mu_split E res.`2]. 
   simplify. smt. smt.
   have : 0%r <=
 bigi predT
   (fun (i : int) =>
-     (1%r - Pr[W0(Sim1,D).run(p,w,aux) @ &m : E res.`2]) ^ i *
-     Pr[W0(Sim1,D).run(p,w,aux) @ &m : E res.`2]) 0 ea.
-  apply (big_geq0  Pr[W0(Sim1,D).run(p,w,aux) @ &m : E res.`2] _ ea). smt.
+     (1%r - Pr[W0(Sim1,V,D).run(p,w,aux) @ &m : E res.`2]) ^ i *
+     Pr[W0(Sim1,V,D).run(p,w,aux) @ &m : E res.`2]) 0 ea.
+  apply (big_geq0  Pr[W0(Sim1,V,D).run(p,w,aux) @ &m : E res.`2] _ ea). smt.
   smt. 
-case (Pr[ W0(Sim1,D).run(p,w,aux) @ &m : E res.`2 /\ res.`1] 
-      = Pr[W0(Sim1,D).run(p,w,aux) @ &m : E res.`2]  
+case (Pr[ W0(Sim1,V,D).run(p,w,aux) @ &m : E res.`2 /\ res.`1] 
+      = Pr[W0(Sim1,V,D).run(p,w,aux) @ &m : E res.`2]  
         * (zkp + eps')).
 progress. rewrite /(\o).
 rewrite zk_step2. 
 rewrite H. simplify.
 have : bigi predT
   (fun (i : int) =>
-     Pr[W0(Sim1,D).run(p,w,aux) @ &m : ! E res.`2] ^ i *
-     (Pr[W0(Sim1,D).run(p,w,aux) @ &m : E res.`2] *
+     Pr[W0(Sim1,V,D).run(p,w,aux) @ &m : ! E res.`2] ^ i *
+     (Pr[W0(Sim1,V,D).run(p,w,aux) @ &m : E res.`2] *
       (zkp + eps'))) 0 ea =
 coeff * zkp + coeff * eps'.
 rewrite coeffeq.
@@ -171,8 +179,8 @@ rewrite - big_split.
 simplify. smt.
 timeout 20. smt.
 move => H5.
-have : Pr[ W0(Sim1,D).run(p,w,aux) @ &m : E res.`2 /\ res.`1] 
-        = Pr[W0(Sim1,D).run(p,w,aux) @ &m : E res.`2]  
+have : Pr[ W0(Sim1,V,D).run(p,w,aux) @ &m : E res.`2 /\ res.`1] 
+        = Pr[W0(Sim1,V,D).run(p,w,aux) @ &m : E res.`2]  
           * (zkp - eps').
 smt.
 progress. rewrite /(\o).
@@ -180,8 +188,8 @@ rewrite zk_step2.
 rewrite H. simplify.
 have : bigi predT
   (fun (i : int) =>
-     Pr[W0(Sim1,D).run(p,w,aux) @ &m : ! E res.`2] ^ i *
-     (Pr[W0(Sim1,D).run(p,w,aux) @ &m : E res.`2] *
+     Pr[W0(Sim1,V,D).run(p,w,aux) @ &m : ! E res.`2] ^ i *
+     (Pr[W0(Sim1,V,D).run(p,w,aux) @ &m : E res.`2] *
       (zkp - eps'))) 0 ea =
 coeff * zkp - coeff * eps'.
 rewrite coeffeq.
@@ -194,46 +202,46 @@ qed.
 
 
 local lemma zk_non_final &m p  eps ea coeff zkp w aux:
-   `|Pr[ W0(Sim1,D).run(p,w,aux) @ &m : E res.`2 /\  res.`1] / Pr[W0(Sim1,D).run(p,w,aux) @ &m : E res.`2] 
+   `|Pr[ W0(Sim1,V,D).run(p,w,aux) @ &m : E res.`2 /\  res.`1] / Pr[W0(Sim1,V,D).run(p,w,aux) @ &m : E res.`2] 
         - zkp| <= eps
-  => 0%r < Pr[W0(Sim1,D).run(p,w,aux) @ &m : E res.`2] 
+  => 0%r < Pr[W0(Sim1,V,D).run(p,w,aux) @ &m : E res.`2] 
   => 0%r <= eps                 (* not needed *)
   => coeff = big predT
-               (fun i => Pr[W0(Sim1,D).run(p,w,aux) @ &m : !E res.`2] ^ i 
-                          * Pr[ W0(Sim1,D).run(p,w,aux) @ &m : E res.`2])
+               (fun i => Pr[W0(Sim1,V,D).run(p,w,aux) @ &m : !E res.`2] ^ i 
+                          * Pr[ W0(Sim1,V,D).run(p,w,aux) @ &m : E res.`2])
                (range 0 ea) 
-  => `|Pr[ Iter(Sim1, D).run((fevent, p, w,aux,ea,E) ) 
+  => `|Pr[ Iter(Sim1, V,D).run((fevent, p, w,aux,ea,E) ) 
            @ &m : E res.`2 /\ res.`1 ]  
               - coeff * zkp| <= eps.
 proof. move => H1 H2 H3 H4. 
 have ->: 
-  Pr[Iter(Sim1, D).run(fevent, p, w, aux,ea, E) @ &m :
+  Pr[Iter(Sim1, V,D).run(fevent, p, w, aux,ea, E) @ &m :
      E res.`2 /\ res.`1]
-  = Pr[ W1(Sim1,D).run((E,p,1,ea,(fevent,witness)), w, aux) 
+  = Pr[ W1(Sim1,V,D).run((E,(p,aux),1,ea,(fevent,witness)), w) 
            @ &m : E res.`2 /\ res.`1 ] .  
  byequiv (_: _==> ={res}). proc*.
-inline Iter(Sim1, D).run. sp. wp. 
-call (_: ={glob Sim1, glob D}). simplify. sim. 
+inline Iter(Sim1, V,D).run. sp. wp. 
+call (_: ={glob Sim1, glob D, glob V}). simplify. sim.  
 skip. smt. auto. auto.
 have : coeff <= 1%r. 
 rewrite H4.
-have ->: Pr[W0(Sim1,D).run(p,w,aux) @ &m : ! E res.`2]
-  = 1%r - Pr[W0(Sim1,D).run(p,w,aux) @ &m :  E res.`2].
-  have ->: 1%r = Pr[W0(Sim1,D).run(p,w,aux) @ &m :  true].
+have ->: Pr[W0(Sim1,V,D).run(p,w,aux) @ &m : ! E res.`2]
+  = 1%r - Pr[W0(Sim1,V,D).run(p,w,aux) @ &m :  E res.`2].
+  have ->: 1%r = Pr[W0(Sim1,V,D).run(p,w,aux) @ &m :  true].
   byphoare. proc.  call D_ll. call Sim1_ll.  auto. auto. auto.
-  have ->: Pr[W0(Sim1,D).run(p,w,aux) @ &m : true] = Pr[W0(Sim1,D).run(p,w,aux) @ &m : E res.`2]
-   + Pr[W0(Sim1,D).run(p,w,aux) @ &m : !E res.`2]. rewrite Pr[mu_split E res.`2]. 
+  have ->: Pr[W0(Sim1,V,D).run(p,w,aux) @ &m : true] = Pr[W0(Sim1,V,D).run(p,w,aux) @ &m : E res.`2]
+   + Pr[W0(Sim1,V,D).run(p,w,aux) @ &m : !E res.`2]. rewrite Pr[mu_split E res.`2]. 
   simplify. smt. smt.
   have : 
 bigi predT
   (fun (i : int) =>
-     (1%r - Pr[W0(Sim1,D).run(p,w,aux) @ &m : E res.`2]) ^ i *
-     Pr[W0(Sim1,D).run(p,w,aux) @ &m : E res.`2]) 0 ea <= 1%r.
-  apply (big_leq1  Pr[W0(Sim1,D).run(p,w,aux) @ &m : E res.`2] _ ea). smt.
+     (1%r - Pr[W0(Sim1,V,D).run(p,w,aux) @ &m : E res.`2]) ^ i *
+     Pr[W0(Sim1,V,D).run(p,w,aux) @ &m : E res.`2]) 0 ea <= 1%r.
+  apply (big_leq1  Pr[W0(Sim1,V,D).run(p,w,aux) @ &m : E res.`2] _ ea). smt.
   smt.
 move => H6.
-have : exists eps', 0%r <= eps' <= eps /\ `|Pr[W1(Sim1,D).run((E, p, 1, ea,
-                 (fevent, witness)),w,aux) @ &m :
+have : exists eps', 0%r <= eps' <= eps /\ `|Pr[W1(Sim1,V,D).run((E, (p,aux), 1, ea,
+                 (fevent, witness)),w) @ &m :
      E res.`2 /\ res.`1] -
   coeff * zkp| 
   = coeff * eps'.
@@ -248,20 +256,20 @@ qed.
 
 
 local lemma zk_almost_final &m p w eps ea coeff zkp aux:
-   `|Pr[ W0(Sim1,D).run(p,w,aux) @ &m : E res.`2 /\ res.`1] 
-        / Pr[W0(Sim1,D).run(p,w,aux) @ &m : E res.`2] 
+   `|Pr[ W0(Sim1,V,D).run(p,w,aux) @ &m : E res.`2 /\ res.`1] 
+        / Pr[W0(Sim1,V,D).run(p,w,aux) @ &m : E res.`2] 
         - zkp| <= eps
-  => 0%r < Pr[W0(Sim1,D).run(p,w,aux) @ &m : E res.`2] 
+  => 0%r < Pr[W0(Sim1,V,D).run(p,w,aux) @ &m : E res.`2] 
   => coeff = big predT
-               (fun i => Pr[W0(Sim1,D).run(p,w,aux) @ &m : !E res.`2] ^ i 
-                         * Pr[ W0(Sim1,D).run(p,w,aux) @ &m : E res.`2])
+               (fun i => Pr[W0(Sim1,V,D).run(p,w,aux) @ &m : !E res.`2] ^ i 
+                         * Pr[ W0(Sim1,V,D).run(p,w,aux) @ &m : E res.`2])
                (range 0 ea) 
-  => `|Pr[ Iter(Sim1, D).run((fevent, p,w,aux,ea,E)) 
+  => `|Pr[ Iter(Sim1, V,D).run((fevent, p,w,aux,ea,E)) 
            @ &m : E res.`2 /\ res.`1 ]  
          - zkp| <= eps + (1%r - coeff).
 proof.
 move => H1 H2 H3.
-have ie1 : `|Pr[ Iter(Sim1, D).run(fevent, p,w,aux,ea,E) 
+have ie1 : `|Pr[ Iter(Sim1, V,D).run(fevent, p,w,aux,ea,E) 
            @ &m : E res.`2 /\  res.`1 ]  
          - coeff * zkp| <= eps.
 apply (zk_non_final &m p eps ea coeff zkp);auto. smt.
@@ -271,121 +279,121 @@ qed.
 
 
 local lemma zk_final &m p w eps ea zkp aux:
-   `|Pr[ W0(Sim1,D).run(p,w,aux) @ &m : E res.`2 /\ res.`1] 
-        / Pr[W0(Sim1,D).run(p,w,aux) @ &m : E res.`2] 
+   `|Pr[ W0(Sim1,V,D).run(p,w,aux) @ &m : E res.`2 /\ res.`1] 
+        / Pr[W0(Sim1,V,D).run(p,w,aux) @ &m : E res.`2] 
         - zkp| <= eps
   => 0 <= ea
-  => `|Pr[ Iter(Sim1, D).run(fevent,p,w,aux,ea,E) 
+  => `|Pr[ Iter(Sim1, V,D).run(fevent,p,w,aux,ea,E) 
            @ &m : E res.`2 /\ res.`1 ]  
          - zkp| 
-           <= eps + Pr[W0(Sim1,D).run(p,w,aux) @ &m : !E res.`2] ^ ea.
+           <= eps + Pr[W0(Sim1,V,D).run(p,w,aux) @ &m : !E res.`2] ^ ea.
 proof. 
-case (0%r = Pr[W0(Sim1,D).run(p,w,aux) @ &m : E res.`2]).
+case (0%r = Pr[W0(Sim1,V,D).run(p,w,aux) @ &m : E res.`2]).
 move => r. rewrite - r. simplify. progress.
-have <-: 1%r = Pr[W0(Sim1,D).run(p,w,aux) @ &m : ! E res.`2]. 
-  have ->: 1%r = Pr[W0(Sim1,D).run(p,w,aux) @ &m : true ].  
+have <-: 1%r = Pr[W0(Sim1,V,D).run(p,w,aux) @ &m : ! E res.`2]. 
+  have ->: 1%r = Pr[W0(Sim1,V,D).run(p,w,aux) @ &m : true ].  
   byphoare. proc. call D_ll. call Sim1_ll. auto. auto. auto.
   rewrite Pr[mu_split (E res.`2)]. simplify. rewrite - r. 
   simplify. auto.
 have ->: 1%r ^ ea = 1%r. smt.
 smt.
 progress.
-have f : 0%r < Pr[W0(Sim1,D).run(p,w,aux) @ &m : E res.`2].  smt.
-have ->: Pr[W0(Sim1,D).run(p,w,aux) @ &m : !E res.`2] ^ ea
- = 1%r - (1%r - Pr[W0(Sim1,D).run(p,w,aux) @ &m : !E res.`2] ^ ea).
+have f : 0%r < Pr[W0(Sim1,V,D).run(p,w,aux) @ &m : E res.`2].  smt.
+have ->: Pr[W0(Sim1,V,D).run(p,w,aux) @ &m : !E res.`2] ^ ea
+ = 1%r - (1%r - Pr[W0(Sim1,V,D).run(p,w,aux) @ &m : !E res.`2] ^ ea).
 smt.
 rewrite - big_formula_p. smt. auto. progress.
-have ->: (1%r - Pr[W0(Sim1,D).run(p,w,aux) @ &m : ! E res.`2])
- = Pr[W0(Sim1,D).run(p,w,aux) @ &m : E res.`2].
-have ->: 1%r = Pr[W0(Sim1,D).run(p,w,aux) @ &m :  true].
+have ->: (1%r - Pr[W0(Sim1,V,D).run(p,w,aux) @ &m : ! E res.`2])
+ = Pr[W0(Sim1,V,D).run(p,w,aux) @ &m : E res.`2].
+have ->: 1%r = Pr[W0(Sim1,V,D).run(p,w,aux) @ &m :  true].
 byphoare.
 proc.  call D_ll. call Sim1_ll. auto. auto. auto.
-have ->: Pr[W0(Sim1,D).run(p,w,aux) @ &m : true] = Pr[W0(Sim1,D).run(p,w,aux) @ &m : ! E res.`2]
- + Pr[W0(Sim1,D).run(p,w,aux) @ &m : E res.`2]. rewrite Pr[mu_split ! E res.`2].
+have ->: Pr[W0(Sim1,V,D).run(p,w,aux) @ &m : true] = Pr[W0(Sim1,V,D).run(p,w,aux) @ &m : ! E res.`2]
+ + Pr[W0(Sim1,V,D).run(p,w,aux) @ &m : E res.`2]. rewrite Pr[mu_split ! E res.`2].
 simplify. smt. smt.
 apply (zk_almost_final &m);auto.
 qed.
 
 
 lemma zk_final_le &m p w p0 eps ea zkp aux:
-   `|Pr[ W0(Sim1,D).run(p,w,aux) @ &m : E res.`2 /\ res.`1] 
-        / Pr[W0(Sim1,D).run(p,w,aux) @ &m : E res.`2] - zkp| <= eps
+   `|Pr[ W0(Sim1,V,D).run(p,w,aux) @ &m : E res.`2 /\ res.`1] 
+        / Pr[W0(Sim1,V,D).run(p,w,aux) @ &m : E res.`2] - zkp| <= eps
   => 0 <= ea
-  => Pr[W0(Sim1,D).run(p,w,aux) @ &m : E res.`2] >= p0
-  => `|Pr[ Iter(Sim1, D).run(fevent,p,w,aux,ea,E) 
+  => Pr[W0(Sim1,V,D).run(p,w,aux) @ &m : E res.`2] >= p0
+  => `|Pr[ Iter(Sim1, V,D).run(fevent,p,w,aux,ea,E) 
            @ &m : E res.`2 /\ res.`1 ] - zkp| 
               <= eps + (1%r-p0) ^ ea.
 progress.
 have fff : p0 <= 1%r. smt.
-have f1 : `|Pr[ Iter(Sim1, D).run(fevent, p,w,aux,ea,E) 
+have f1 : `|Pr[ Iter(Sim1, V,D).run(fevent, p,w,aux,ea,E) 
            @ &m : E res.`2 /\ res.`1 ]  
          - zkp| 
-      <= eps + (1%r - Pr[W0(Sim1,D).run(p,w,aux) @ &m : E res.`2] )^ea.
-have ->: (1%r - Pr[W0(Sim1,D).run(p,w,aux) @ &m : E res.`2] ) = 
-  (Pr[W0(Sim1,D).run(p,w,aux) @ &m : !E res.`2] ). 
-have ->: 1%r = Pr[W0(Sim1,D).run(p,w,aux) @ &m :  true].
+      <= eps + (1%r - Pr[W0(Sim1,V,D).run(p,w,aux) @ &m : E res.`2] )^ea.
+have ->: (1%r - Pr[W0(Sim1,V,D).run(p,w,aux) @ &m : E res.`2] ) = 
+  (Pr[W0(Sim1,V,D).run(p,w,aux) @ &m : !E res.`2] ). 
+have ->: 1%r = Pr[W0(Sim1,V,D).run(p,w,aux) @ &m :  true].
 byphoare. proc. call D_ll. call Sim1_ll. auto. auto. auto.
-have ->: Pr[W0(Sim1,D).run(p,w,aux) @ &m : true] = Pr[W0(Sim1,D).run(p,w,aux) @ &m : ! E res.`2]
- + Pr[W0(Sim1,D).run(p,w,aux) @ &m : E res.`2]. rewrite Pr[mu_split ! E res.`2]. 
+have ->: Pr[W0(Sim1,V,D).run(p,w,aux) @ &m : true] = Pr[W0(Sim1,V,D).run(p,w,aux) @ &m : ! E res.`2]
+ + Pr[W0(Sim1,V,D).run(p,w,aux) @ &m : E res.`2]. rewrite Pr[mu_split ! E res.`2]. 
 simplify. smt. smt.
 apply (zk_final &m).
 have f2 : 
- (1%r - Pr[W0(Sim1,D).run(p,w,aux) @ &m : E res.`2]) <= (1%r - p0). smt.
-have f3 : (1%r - Pr[W0(Sim1,D).run(p,w,aux) @ &m : E res.`2]) ^ ea <= (1%r - p0) ^ ea.
+ (1%r - Pr[W0(Sim1,V,D).run(p,w,aux) @ &m : E res.`2]) <= (1%r - p0). smt.
+have f3 : (1%r - Pr[W0(Sim1,V,D).run(p,w,aux) @ &m : E res.`2]) ^ ea <= (1%r - p0) ^ ea.
 apply multn2;auto. smt. auto. auto. auto. smt.
 qed.
 
 
 
 lemma zk_final_clean &m p w p0 eps ea zkp aux:
-   `|Pr[ W0(Sim1,D).run(p,w,aux) @ &m : E res.`2 /\ res.`1] 
-        / Pr[W0(Sim1,D).run(p,w,aux) @ &m : E res.`2] - zkp| <= eps
+   `|Pr[ W0(Sim1,V,D).run(p,w,aux) @ &m : E res.`2 /\ res.`1] 
+        / Pr[W0(Sim1,V,D).run(p,w,aux) @ &m : E res.`2] - zkp| <= eps
   => 0 <= ea
-  => Pr[W0(Sim1,D).run(p,w,aux) @ &m : E res.`2] >= p0
-  => `|Pr[ Iter(Sim1, D).run(fevent,p,w,aux,ea,E) 
+  => Pr[W0(Sim1,V,D).run(p,w,aux) @ &m : E res.`2] >= p0
+  => `|Pr[ Iter(Sim1, V,D).run(fevent,p,w,aux,ea,E) 
            @ &m : res.`1 ] - zkp| 
               <= eps + 2%r * (1%r-p0) ^ ea.
 proof.  progress.
-have bf :  `|Pr[ Iter(Sim1, D).run(fevent,p,w,aux,ea,E) 
+have bf :  `|Pr[ Iter(Sim1, V,D).run(fevent,p,w,aux,ea,E) 
            @ &m : res.`1 ] - zkp| 
               <= (eps + (1%r-p0) ^ ea ) +
-(Pr[ Iter(Sim1, D).run(fevent,p,w,aux,ea,E) 
+(Pr[ Iter(Sim1, V,D).run(fevent,p,w,aux,ea,E) 
            @ &m : !E res.`2]).
-have f1 : `|Pr[ Iter(Sim1, D).run(fevent,p,w,aux,ea,E) 
+have f1 : `|Pr[ Iter(Sim1, V,D).run(fevent,p,w,aux,ea,E) 
            @ &m : E res.`2 /\ res.`1 ] - zkp| 
               <= eps + (1%r-p0) ^ ea.
 apply (zk_final_le &m p w p0 eps ea zkp aux);auto.
-apply (kkk Pr[Iter(Sim1, D).run(fevent, p, w, aux, ea, E) @ &m : res.`1]
-Pr[Iter(Sim1, D).run(fevent, p, w, aux, ea, E) @ &m :
+apply (kkk Pr[Iter(Sim1, V,D).run(fevent, p, w, aux, ea, E) @ &m : res.`1]
+Pr[Iter(Sim1, V,D).run(fevent, p, w, aux, ea, E) @ &m :
          E res.`2 /\ res.`1]). smt.
 rewrite Pr[mu_split E res.`2] .
-have ->: Pr[Iter(Sim1, D).run(fevent, p, w, aux, ea, E) @ &m : res.`1 /\ E res.`2]
- = Pr[Iter(Sim1, D).run(fevent, p, w, aux, ea, E) @ &m : E res.`2 /\ res.`1 ].
+have ->: Pr[Iter(Sim1, V,D).run(fevent, p, w, aux, ea, E) @ &m : res.`1 /\ E res.`2]
+ = Pr[Iter(Sim1, V,D).run(fevent, p, w, aux, ea, E) @ &m : E res.`2 /\ res.`1 ].
 smt.
 smt.
 auto.  
 clear H.
-have bf2 : Pr[Iter(Sim1, D).run(fevent, p, w, aux, ea, E) @ &m : ! E res.`2]
+have bf2 : Pr[Iter(Sim1, V,D).run(fevent, p, w, aux, ea, E) @ &m : ! E res.`2]
   <= (1%r - p0) ^ ea.
-  have bf3: Pr[W0(Sim1, D).run(p, w, aux) @ &m : !E res.`2] <= 1%r - p0.
-    have -> : 1%r = Pr[W0(Sim1, D).run(p, w, aux) @ &m : true]. byphoare.
+  have bf3: Pr[W0(Sim1, V,D).run(p, w, aux) @ &m : !E res.`2] <= 1%r - p0.
+    have -> : 1%r = Pr[W0(Sim1, V,D).run(p, w, aux) @ &m : true]. byphoare.
     proc. call D_ll. call Sim1_ll. auto. auto. auto.
-       have : Pr[W0(Sim1, D).run(p, w, aux) @ &m : true] 
-                - Pr[W0(Sim1, D).run(p, w, aux) @ &m : !E res.`2] 
-                 = Pr[W0(Sim1, D).run(p, w, aux) @ &m : E res.`2]. 
+       have : Pr[W0(Sim1, V,D).run(p, w, aux) @ &m : true] 
+                - Pr[W0(Sim1, V,D).run(p, w, aux) @ &m : !E res.`2] 
+                 = Pr[W0(Sim1, V,D).run(p, w, aux) @ &m : E res.`2]. 
     rewrite Pr[mu_split E res.`2]. simplify. smt.
 smt.
-  have ->: Pr[Iter(Sim1, D).run(fevent, p, w, aux, ea, E) @ &m : ! E res.`2] 
-     = Pr[ W(Sim1).whp(E,p,1,ea,(fevent,witness)) @ &m : ! E res ].
-   byequiv. proc*.  inline Iter(Sim1, D).run. sp. wp. inline Iter(Sim1, D).WI.run.
+  have ->: Pr[Iter(Sim1, V,D).run(fevent, p, w, aux, ea, E) @ &m : ! E res.`2] 
+     = Pr[ W(Sim1(V)).whp(E,(p,aux),1,ea,(fevent,witness)) @ &m : ! E res ].
+   byequiv. proc*.  inline Iter(Sim1, V,D).run. sp. wp. inline Iter(Sim1, V,D).WI.run.
  sp. wp. call {1} D_ll. 
   conseq (_: _==> r1{1} = r0{2}). smt.
-call (_: ={glob Sim1}).  sim. skip. progress. auto. auto.
-apply (final_zz_le Sim1 Sim1_ll &m). smt. auto. 
-have ->: Pr[Sim1.run(p) @ &m : ! E res] 
-  = Pr[W0(Sim1, D).run(p, w, aux) @ &m : ! E res.`2].
-byequiv. proc*. inline*. wp. sp. call {2} D_ll. call (_:true).
-skip. progress. auto. auto. auto.
+call (_: ={glob Sim1, glob V}).  sim. skip. progress. auto. auto.
+apply (final_zz_le (Sim1(V)) Sim1_ll &m). smt. auto. 
+have ->: Pr[Sim1(V).run(p,aux) @ &m : ! E res] 
+  = Pr[W0(Sim1, V,D).run(p, w, aux) @ &m : ! E res.`2].
+byequiv. proc*. inline*. wp. sp. call {2} D_ll. call (_: ={glob V}).
+sim.    sim.  skip. progress. auto. auto. auto.
 smt.
 qed.
 
